\documentclass[12pt]{article}
\usepackage[utf8]{inputenc}
\usepackage{amsmath}
\usepackage{amssymb}

\begin{document}


\begin{enumerate}
    \item Show the following identities using the Euler Product:
    \begin{equation}
        \sum \frac{\phi(n)}{n^{s}} = \frac{\zeta(1-s)}{\zeta(s)}
    \end{equation}
    \begin{equation}
        \sum \frac{\tau(n)}{n^{s}} = \zeta(s)^{2}
    \end{equation}
    \begin{equation}
        \sum \frac{\sigma(n)}{n^{s}} = \zeta(s-1)\zeta(s)
    \end{equation}
    \begin{equation}
        \sum \frac{\sigma_{k}(n)}{n^{s}} = \zeta(s-k)\zeta(s)
    \end{equation}
    \begin{equation}
        \sum \frac{\mu(n)}{n^{s}} = \frac{1}{\zeta(s)}.
    \end{equation}
    Recall $\phi$ is the totient function, $\tau$ is the number of divisors, $\sigma$ is the sum of divisors, $\sigma_{k}$ is the sum of divisors to the k-th power, and $\mu$ is the Mobius inversion function.
    \item Use (5) to show
    \begin{equation}
        \sum_{d \mid n}b_{d} \cdot \mu(\frac{n}{d}) = a_{n}
    \end{equation}
    if
    \begin{equation*}
        \sum_{d \mid n}a_{d} = b_{n}.
    \end{equation*}
    \item Show that
    \begin{equation}
        \sum_{d \mid n} \phi(d) = n. 
    \end{equation}
    Then combine with (6) and (3) to deduce
    \begin{equation}
        \sum \frac{\phi(n)}{n^{s}} = \frac{\zeta(s-1)}{\zeta(s)}.
    \end{equation}
    \item Show that
    \begin{equation}
        \frac{d}{ds}\zeta(s) = -\sum\frac{\log(n)}{n^{s}}
    \end{equation}
    and use the Taylor expansion (which you should verify) of
    \begin{equation}
        \log(1-x) = -x - \frac{x^{2}}{2} ...
    \end{equation}
    to deduce
    \begin{equation}
        \log \zeta(s) = \sum_{p}(p^{-2} + \frac{p^{-2s}}{2} + ...).
    \end{equation}
    \item From (11), conclude
    \begin{equation}
        \frac{\zeta'(s)}{\zeta(s)} 
        = -\sum_{p}\sum_{m}\frac{\log(p)}{p^{ms}}
        = -\sum_{n}\frac{\Lambda(n^{s})}{n^{s}}
    \end{equation}
    where $\Lambda(s) = \log(p)$ if $s = p^{k}$.
    \item Prove the equation
    \begin{equation}
        \Lambda(n)\log(n) + \sum_{d \mid n}\Lambda(d)\Lambda(\frac{n}{d})
        = \sum_{d \mid n} \mu(d) \cdot \log^{2}(\frac{n}{d})
    \end{equation}
    by noting the following identities:
    \begin{equation}
        \sum n^{-s}\sum_{d \mid n} \mu(d) \cdot \log^{2}(\frac{n}{d}) = \frac{\zeta''(s)}{\zeta(s)}
    \end{equation}
    \begin{equation}
        \sum n^{-s} \Lambda(n)\log(n) =
        - \frac{d}{ds}(\frac{\zeta'(s)}{\zeta(s)})
    \end{equation}
    \begin{equation}
        \sum n^{-s} \sum_{d \mid n}\Lambda(d)\Lambda(\frac{n}{d}) =
        (\frac{\zeta'(s)}{\zeta(s)})^{2}
    \end{equation}
    the last two of which come from (12).
\end{enumerate}

\end{document}